LeanSAT/Reflect/BVExpr/BitBlast/Lemmas/Add.lean
@@ -38,28 +38,85 @@ theorem denote_mkFullAdderCarry (assign : Assignment) (aig : AIG BVBit) (input :
   simp only [mkFullAdderCarry, Ref_cast', Int.reduceNeg, denote_mkOrCached,
     LawfulOperator.denote_input_entry, denote_mkAndCached, denote_projected_entry',
     denote_mkXorCached, denote_projected_entry]
-  -- Without conv mode this timeouts
-  conv =>
-    lhs
-    lhs
-    rhs
-    rw [LawfulOperator.denote_mem_prefix (f := mkXorCached) (h := input.cin.hgate)]
-  conv =>
-    lhs
-    rhs
-    lhs
-    rw [LawfulOperator.denote_mem_prefix (f := mkAndCached)]
-    rw [LawfulOperator.denote_mem_prefix (f := mkXorCached) (h := input.lhs.hgate)]
-  conv =>
-    lhs
-    rhs
-    rhs
-    rw [LawfulOperator.denote_mem_prefix (f := mkAndCached)]
-    rw [LawfulOperator.denote_mem_prefix (f := mkXorCached) (h := input.rhs.hgate)]
+  rw [LawfulOperator.denote_mem_prefix (f := mkXorCached) (h := input.cin.hgate)]
+  rw [LawfulOperator.denote_mem_prefix (f := mkAndCached)]
+  rw [LawfulOperator.denote_mem_prefix (f := mkXorCached) (h := input.lhs.hgate)]
+  rw [LawfulOperator.denote_mem_prefix (f := mkAndCached)]
+  rw [LawfulOperator.denote_mem_prefix (f := mkXorCached) (h := input.rhs.hgate)]
 
--- TODO: additional assumption about cin
--- Proof idea: show that go always pulls through something that is equiv to BitVec.carry at the
--- next idx. In particular assuming that the thing it was given was BitVec.carry at the current
+theorem mkFullAdder_denote_mem_prefix (aig : AIG BVBit) (input : FullAdderInput aig) (start : Nat)
+    (hstart)
+  : ⟦
+      (mkFullAdder aig input).aig,
+      ⟨start, by apply Nat.lt_of_lt_of_le; exact hstart; apply FullAdderOutput.hle⟩,
+      assign
+    ⟧
+      =
+    ⟦aig, ⟨start, hstart⟩, assign⟧ := by
+  unfold mkFullAdder
+  dsimp
+  rw [AIG.LawfulOperator.denote_mem_prefix (f := mkFullAdderCarry)]
+  rw [AIG.LawfulOperator.denote_mem_prefix (f := mkFullAdderOut)]
+
+theorem go_denote_mem_prefix (aig : AIG BVBit) (curr : Nat) (hcurr : curr ≤ w) (cin : Ref aig)
+    (s : AIG.RefStream aig curr) (lhs rhs : AIG.RefStream aig w) (start : Nat) (hstart)
+  : ⟦
+      (go aig curr hcurr cin s lhs rhs).aig,
+      ⟨start, by apply Nat.lt_of_lt_of_le; exact hstart; apply go_le_size⟩,
+      assign
+    ⟧
+      =
+    ⟦aig, ⟨start, hstart⟩, assign⟧ := by
+  apply denote.eq_of_aig_eq (entry := ⟨aig, start,hstart⟩)
+  apply IsPrefix.of
+  . intros
+    apply go_decl_eq
+  . intros
+    apply go_le_size
+
+theorem go_getRef_aux (aig : AIG BVBit) (curr : Nat) (hcurr : curr ≤ w) (cin : Ref aig)
+    (s : AIG.RefStream aig curr) (lhs rhs : AIG.RefStream aig w)
+    -- The hfoo here is a trick to make the dependent type gods happy
+    : ∀ (idx : Nat) (hidx : idx < curr) (hfoo),
+        (go aig curr hcurr cin s lhs rhs).stream.getRef idx (by omega)
+          =
+        (s.getRef idx hidx).cast hfoo := by
+  intro idx hidx
+  generalize hgo : go aig curr hcurr cin s lhs rhs = res
+  unfold go at hgo
+  dsimp at hgo
+  split at hgo
+  . rw [← hgo]
+    intro hfoo
+    rw [go_getRef_aux]
+    rw [AIG.RefStream.getRef_push_ref_lt]
+    . simp only [Ref.cast, Ref.mk.injEq]
+      rw [AIG.RefStream.getRef_cast]
+      . simp
+      . assumption
+    . apply go_le_size
+  . rw [← hgo]
+    simp only [Nat.le_refl, RefStream.getRef, Ref_cast', Ref.mk.injEq, true_implies]
+    congr
+    . omega
+    . simp
+termination_by w - curr
+
+theorem go_getRef (aig : AIG BVBit) (curr : Nat) (hcurr : curr ≤ w) (cin : Ref aig)
+    (s : AIG.RefStream aig curr) (lhs rhs : AIG.RefStream aig w)
+    : ∀ (idx : Nat) (hidx : idx < curr),
+        (go aig curr hcurr cin s lhs rhs).stream.getRef idx (by omega)
+          =
+        (s.getRef idx hidx).cast (by apply go_le_size) := by
+  intros
+  apply go_getRef_aux
+
+theorem _root_.Bool.atLeastTwo_eq_halfAdder (lhsBit rhsBit carry : Bool)
+  : Bool.atLeastTwo lhsBit rhsBit carry
+      =
+    (((xor lhsBit rhsBit) && carry) || (lhsBit && rhsBit)) := by
+  cases lhsBit <;> cases rhsBit <;> cases carry <;> decide
+
 theorem go_eq_eval_getLsb (aig : AIG BVBit) (curr : Nat) (hcurr : curr ≤ w) (cin : Ref aig)
     (s : AIG.RefStream aig curr) (lhs rhs : AIG.RefStream aig w) (assign : Assignment)
     (lhsExpr rhsExpr : BVExpr w)
@@ -83,7 +140,50 @@ theorem go_eq_eval_getLsb (aig : AIG BVBit) (curr : Nat) (hcurr : curr ≤ w) (c
   intro idx hidx1 hidx2
   generalize hgo : go aig curr hcurr cin s lhs rhs = res
   unfold go at hgo
-  sorry
+  dsimp at hgo
+  split at hgo
+  . next hlt =>
+    cases Nat.eq_or_lt_of_le hidx2 with
+    | inl heq =>
+      rw [← hgo]
+      rw [go_getRef (hidx := by omega)]
+      rw [AIG.RefStream.getRef_push_ref_eq' (hidx := by rw [heq])]
+      simp only [← heq]
+      rw [go_denote_mem_prefix]
+      . unfold mkFullAdder
+        simp [hcin]
+      . simp only [Ref_cast']
+        apply Ref.hgate
+    | inr hlt =>
+      rw [← hgo]
+      rw [go_eq_eval_getLsb (lhsExpr := lhsExpr) (rhsExpr := rhsExpr) (curr := curr + 1)]
+      . rw [mkFullAdder_denote_mem_prefix]
+        rw [mkFullAdder_denote_mem_prefix]
+        . simp
+        . simp [Ref.hgate]
+        . simp [Ref.hgate]
+      . intro idx hidx
+        rw [mkFullAdder_denote_mem_prefix]
+        rw [← hleft idx hidx]
+        . simp
+        . simp [Ref.hgate]
+      . intro idx hidx
+        rw [mkFullAdder_denote_mem_prefix]
+        rw [← hright idx hidx]
+        . simp
+        . simp [Ref.hgate]
+      . unfold mkFullAdder
+        simp only [Ref_cast', id_eq, Int.reduceNeg, denote_projected_entry, denote_mkFullAdderCarry,
+          FullAdderInput.lhs_cast, FullAdderInput.rhs_cast, FullAdderInput.cin_cast,
+          BitVec.carry_succ]
+        rw [AIG.LawfulOperator.denote_mem_prefix (f := mkFullAdderOut)]
+        rw [AIG.LawfulOperator.denote_mem_prefix (f := mkFullAdderOut)]
+        rw [AIG.LawfulOperator.denote_mem_prefix (f := mkFullAdderOut)]
+        rw [hleft, hright, hcin]
+        simp [_root_.Bool.atLeastTwo_eq_halfAdder]
+      . omega
+  . omega
+termination_by w - curr
 
 end blastAdd
 
@@ -102,20 +202,17 @@ theorem blastAdd_eq_eval_getLsb (aig : AIG BVBit) (lhs rhs : BVExpr w) (assign :
     unfold blastAdd
     dsimp
     rw [blastAdd.go_eq_eval_getLsb _ 0 (by omega) _ _ _ _ assign lhs rhs _ _]
-    . -- TODO: API lemmas
-      simp [BinaryRefStream.cast]
+    . simp only [BinaryRefStream.lhs_getRef_cast, Ref_cast', BinaryRefStream.rhs_getRef_cast]
       rw [LawfulOperator.denote_mem_prefix (f := mkConstCached)]
       rw [LawfulOperator.denote_mem_prefix (f := mkConstCached)]
     . simp
     . omega
     . intros
-      -- TODO: API lemmas
-      simp [BinaryRefStream.cast]
+      simp only [BinaryRefStream.lhs_getRef_cast, Ref_cast']
       rw [LawfulOperator.denote_mem_prefix (f := mkConstCached)]
       rw [hleft]
     . intros
-      -- TODO: API lemmas
-      simp [BinaryRefStream.cast]
+      simp only [BinaryRefStream.rhs_getRef_cast, Ref_cast']
       rw [LawfulOperator.denote_mem_prefix (f := mkConstCached)]
       rw [hright]
   . assumption
